cleanup mont_mul_add

impl/riscv/rsa_ops.i.dfy
@@ -90,55 +90,84 @@ module rsa_ops {
         sig_it: iter_t,
         rsa: rsa_params)
 
-    predicate mvars_iter_init(iter: iter_t, mem: mem_t, address: int, value: int)
+    predicate mvar_iter_inv(mem: mem_t, iter: iter_t, address: int, index: int, value: int)
     {
         && (address >= 0 ==> iter_inv(iter, mem, address))
         && (value >= 0 ==> to_nat(iter.buff) == value)
-        && iter.index == 0
+        && (index >= 0 ==> iter.index == index)
         && |iter.buff| == NUM_WORDS
     }
 
-    predicate m0d_it_inv(iter: iter_t, mem: mem_t, address: int)
-    {
-        && (address >= 0 ==> iter_inv(iter, mem, address))
-        && iter.index == 0
-        && |iter.buff| == 1
-    }
+    datatype mma_vars = mma_vars(
+        frame_ptr: uint32, // writable
+        iter_a: iter_t,
+        a_i: uint32,
+        i: nat,
+        // d0: uint32,
+        iter_b: iter_t,
+        iter_c: iter_t, // writable
+        iter_n: iter_t
+    )
 
-    predicate mvars_inv(
-        vars: mvars,
+    predicate mma_vars_inv(
+        vars: mma_vars,
         mem: mem_t,
-        x_ptr: int,
-        y_ptr: int,
-        m_ptr: int,
-        rr_ptr: int,
-        sig_ptr: int)
+        n_ptr: int, n_idx: int,
+        c_ptr: int, c_idx: int,
+        b_ptr: int, b_idx: int,
+        rsa: rsa_params)
     {
-        && rsa_params_inv(vars.rsa)
+        && valid_frame_ptr(mem, vars.frame_ptr, 12)
 
-        && mvars_iter_init(vars.x_it, mem, x_ptr, NA)
-        && mvars_iter_init(vars.y_it, mem, y_ptr, NA)
-        && mvars_iter_init(vars.sig_it, mem, sig_ptr, vars.rsa.SIG)
-        && mvars_iter_init(vars.m_it, mem, m_ptr, vars.rsa.M)
-        && mvars_iter_init(vars.rr_it, mem, rr_ptr, vars.rsa.RR)
+        && mvar_iter_inv(mem, vars.iter_a, -1, vars.i, NA)
+        && vars.i < NUM_WORDS
+        && vars.iter_a.buff[vars.i] == vars.a_i
+        && mvar_iter_inv(mem, vars.iter_n, n_ptr, n_idx, rsa.M)
+        && mvar_iter_inv(mem, vars.iter_c, c_ptr, c_idx, NA)
+        && mvar_iter_inv(mem, vars.iter_b, b_ptr, b_idx, NA)
+
+        && vars.iter_c.base_addr != vars.iter_a.base_addr
+        && vars.iter_c.base_addr != vars.iter_n.base_addr
+        && vars.iter_c.base_addr != vars.iter_b.base_addr
+        && vars.iter_c.base_addr != vars.frame_ptr
+
+        && vars.frame_ptr != vars.iter_a.base_addr
+        && vars.frame_ptr != vars.iter_n.base_addr
+        && vars.frame_ptr != vars.iter_b.base_addr
+
+        && rsa_params_inv(rsa)
     }
 
-    predicate mvars_init(
-        vars: mvars,
-        mem: mem_t,
-        m_ptr: uint32,
-        rr_ptr: uint32,
-        sig_ptr: uint32,
-        out_ptr: uint32)
-    {
-        && rsa_params_inv(vars.rsa)
+    // predicate mvars_inv(
+    //     vars: mvars,
+    //     mem: mem_t,
+    //     x_ptr: int,
+    //     y_ptr: int,
+    //     m_ptr: int,
+    //     rr_ptr: int,
+    //     sig_ptr: int)
+    // {
+    //     && rsa_params_inv(vars.rsa)
 
-        && mvars_inv(vars, mem, NA, NA, m_ptr, rr_ptr, sig_ptr)
-        && out_ptr in mem
-        && |mem[out_ptr]| == NUM_WORDS
+    //     && mvars_iter_init(vars.x_it, mem, x_ptr, NA)
+    //     && mvars_iter_init(vars.y_it, mem, y_ptr, NA)
+    //     && mvars_iter_init(vars.sig_it, mem, sig_ptr, vars.rsa.SIG)
+    //     && mvars_iter_init(vars.m_it, mem, m_ptr, vars.rsa.M)
+    //     && mvars_iter_init(vars.rr_it, mem, rr_ptr, vars.rsa.RR)
+    // }
 
-        && out_ptr != rr_ptr
-        && out_ptr != m_ptr
-        && out_ptr != sig_ptr
-    }
+    // predicate mvars_init(
+    //     vars: mvars,
+    //     mem: mem_t,
+    //     m_ptr: uint32,
+    //     rr_ptr: uint32,
+    //     sig_ptr: uint32,
+    //     out_ptr: uint32)
+    // {
+    //     && rsa_params_inv(vars.rsa)
+
+    //     && mvars_inv(vars, mem, NA, NA, m_ptr, rr_ptr, sig_ptr)
+
+
+    // }
 }
